wip cleanup specs for falcon

crypto_specs/mq_ntt.i.dfy
@@ -1,62 +1,73 @@
-include "nth_root.dfy"
+include "ntt_twiddle.i.dfy"
 
-abstract module ct_std2rev_model {
+abstract module mq_ntt_i(MQ: ntt_param_s) {
     import opened Seq
 	import opened Power
 	import opened Power2
 	import opened DivMod
 	import opened Mul
 
-	import opened pows_of_2
-    import opened ntt_index
-    import opened nth_root
-    import opened ntt_512_params
-	import opened mq_polys
-    import opened poly_view
+	import opened pow2_s
+	import opened ntt_index
 
-    ghost const x_value: x_fun
+	import MQP = mq_poly_i(MQ)
+	import PV = poly_view_i(MQ)
+	import TWD = ntt_twiddle_i(MQ)
 
-    predicate {:opaque} t_loop_inv(a: n_sized, count: pow2_t, coefficients: n_sized)
+	type elem = MQ.elem
+	type n_elems = MQ.n_elems
+
+	const Q := MQ.Q;
+	const R := MQ.R;
+	const PSI := MQ.PSI;
+	const OMEGA := MQ.OMEGA;
+	const OMEGA_INV := MQ.OMEGA_INV;
+	const R_INV := MQ.R_INV;
+	ghost const N := MQ.N;
+
+    function x_value(i: nat, d: pow2_t): elem
+
+    predicate {:opaque} t_loop_inv(a: n_elems, count: pow2_t, coefficients: n_elems)
         requires 0 <= count.exp <= N.exp;
     {
-        var sz := block_size(count);
-        var points := level_points_view(a, sz);
-        var polys := level_polys(coefficients, sz);
+        var sz := PV.block_size(count);
+        var points := PV.level_points_view(a, sz);
+        var polys := PV.level_polys(coefficients, sz);
         forall i | 0 <= i < count.full ::
-            points_eval_inv(points[i], polys[bit_rev_int(i, count)], x_value, count)
+            PV.points_eval_inv(points[i], polys[bit_rev_int(i, count)], x_value, count)
     }
 
     lemma t_loop_inv_pre_specialized_lemma(points: seq<elem>, poly: seq<elem>, A_i: elem)
         requires poly == [A_i];
         requires points == [A_i];
-        ensures points_eval_inv(points, poly, x_value, N)
+        ensures PV.points_eval_inv(points, poly, x_value, N)
     {
-        assert points_eval_inv(points, poly, x_value, N) by
+        assert PV.points_eval_inv(points, poly, x_value, N) by
         {
-            reveal points_eval_suffix_inv();
+            reveal PV.points_eval_suffix_inv();
             assert N.exp <= N.exp;
-            poly_eval_base_lemma(poly, x_value(0, N));
-            assert points[0] == poly_eval(poly, x_value(0, N));
+            MQP.poly_eval_base_lemma(poly, x_value(0, N));
+            assert points[0] == MQP.poly_eval(poly, x_value(0, N));
         }
     }
 
-    lemma t_loop_inv_pre_lemma(coefficients: n_sized)
+    lemma t_loop_inv_pre_lemma(coefficients: n_elems)
         ensures N.exp <= N.exp; // ??
         ensures t_loop_inv(coefficients, N, coefficients);
     {
         reveal t_loop_inv();
         assert N.exp <= N.exp; // ??
-        var sz := block_size(N);
+        var sz := PV.block_size(N);
         assert sz.full == 1;
         assert sz.exp == 0;
-        var lpoints := level_points_view(coefficients, sz);
-        var lpolys := base_level_polys(coefficients);
+        var lpoints := PV.level_points_view(coefficients, sz);
+        var lpolys :=PV. base_level_polys(coefficients);
 
         forall i | 0 <= i < N.full
-            ensures points_eval_inv(lpoints[i],
+            ensures PV.points_eval_inv(lpoints[i],
                 lpolys[bit_rev_int(i, N)], x_value, N)
         {
-            base_level_polys_lemma(coefficients, i);
+            PV.base_level_polys_lemma(coefficients, i);
             var points := lpoints[i];
             var poly := lpolys[bit_rev_int(i, N)];
             assert poly == [coefficients[i]];
@@ -64,33 +75,33 @@ abstract module ct_std2rev_model {
         }
     }
 
-    predicate ntt_eval_all(a: n_sized, coefficients: n_sized)
+    predicate ntt_eval_all(a: n_elems, coefficients: n_elems)
     {
-        points_eval_inv(a, coefficients, x_value, pow2(0))
+        PV.points_eval_inv(a, coefficients, x_value, pow2(0))
     }
 
-    lemma t_loop_inv_post_lemma(a: n_sized, one: pow2_t, coefficients: n_sized)
+    lemma t_loop_inv_post_lemma(a: n_elems, one: pow2_t, coefficients: n_elems)
         requires one.exp == 0 <= N.exp;
         requires t_loop_inv(a, one, coefficients);
         ensures ntt_eval_all(a, coefficients);
     {
         reveal t_loop_inv();
-        var sz := block_size(one);
-        var points := level_points_view(a, sz);
-        var polys := level_polys(coefficients, sz);
-        Nth_root_lemma();
+        var sz := PV.block_size(one);
+        var points := PV.level_points_view(a, sz);
+        var polys := PV.level_polys(coefficients, sz);
+        MQ.Nth_root_lemma();
         pow2_basics(one);
         assert one.full == 1;
         assert sz == N;
         assert points[0] == a;
 
         assert polys[0] == coefficients by {
-            reveal level_polys();
+            reveal PV.level_polys();
         }
     }
 
     datatype loop_view = loop_view(
-        coefficients: n_sized,
+        coefficients: n_elems,
         lower: seq<seq<elem>>, // lower polys
         higher: seq<seq<elem>>, // higher polys
         hsize: pow2_t)
@@ -98,9 +109,9 @@ abstract module ct_std2rev_model {
         predicate loop_view_wf()
         {
             && 1 <= hsize.exp <= N.exp
-            && unifromly_sized(higher, hsize)
-		    && higher == level_polys(coefficients, hsize)
-		    && lower == level_polys(coefficients, pow2_half(hsize))
+            && PV.unifromly_sized(higher, hsize)
+		    && higher == PV.level_polys(coefficients, hsize)
+		    && lower == PV.level_polys(coefficients, pow2_half(hsize))
         }
 
         function lsize(): (r: pow2_t)
@@ -118,14 +129,14 @@ abstract module ct_std2rev_model {
         function lcount(): (r: pow2_t)
             requires loop_view_wf();
         {
-            block_count(lsize())
+            PV.block_count(lsize())
         }
 
         function hcount(): (r: pow2_t)
             requires loop_view_wf();
             ensures r.full <= N.full;
         {
-            var r := block_count(hsize);
+            var r := PV.block_count(hsize);
             assert r.full <= N.full by {
                 reveal Pow2();
                 LemmaPowIncreases(2, r.exp, N.exp);
@@ -140,8 +151,8 @@ abstract module ct_std2rev_model {
             ensures lcount().full * lsize().full
                 == hcount().full * hsize.full == N.full;
         {
-            Nth_root_lemma();
-            block_count_half_lemma(hsize);
+            MQ.Nth_root_lemma();
+            PV.block_count_half_lemma(hsize);
         }
 
         // lemma size_count_bound_lemma()
@@ -164,138 +175,138 @@ abstract module ct_std2rev_model {
         //         hsize)
         // }
 
-        predicate {:opaque} j_loop_higher_inv(a: n_sized, hcount: pow2_t, j: nat)
+        predicate {:opaque} j_loop_higher_inv(a: n_elems, hcount: pow2_t, j: nat)
             requires hcount.exp <= N.exp;
             requires loop_view_wf();
-            requires hsize == block_size(hcount);
+            requires hsize == PV.block_size(hcount);
         {
-            && var hpoints := level_points_view(a, hsize);
+            && var hpoints := PV.level_points_view(a, hsize);
             && (forall i | 0 <= i < hcount.full ::
-                points_eval_prefix_inv(hpoints[i], higher[bit_rev_int(i, hcount)], x_value, 2*j, hcount))
+                PV.points_eval_prefix_inv(hpoints[i], higher[bit_rev_int(i, hcount)], x_value, 2*j, hcount))
         }
 
-        predicate {:opaque} j_loop_lower_inv(a: n_sized, hcount: pow2_t, j: nat)
+        predicate {:opaque} j_loop_lower_inv(a: n_elems, hcount: pow2_t, j: nat)
             requires hcount.exp <= N.exp;
             requires loop_view_wf();
-            requires hsize == block_size(hcount);
+            requires hsize == PV.block_size(hcount);
         {
             && var lcount := lcount();
-            && var lpoints := level_points_view(a, lsize());
+            && var lpoints := PV.level_points_view(a, lsize());
             && (forall i | 0 <= i < lcount.full ::
-                points_eval_suffix_inv(lpoints[i], lower[bit_rev_int(i, lcount)], x_value, j, lcount))
+                PV.points_eval_suffix_inv(lpoints[i], lower[bit_rev_int(i, lcount)], x_value, j, lcount))
         }
 
-        predicate j_loop_inv(a: n_sized, hcount: pow2_t, j: nat)
+        predicate j_loop_inv(a: n_elems, hcount: pow2_t, j: nat)
         {
             && loop_view_wf()
             && hcount.exp <= N.exp
-            && hsize == block_size(hcount)
+            && hsize == PV.block_size(hcount)
             && j <= lsize().full
             && j_loop_higher_inv(a, hcount, j)
             && j_loop_lower_inv(a, hcount, j)
         }
 
-        predicate {:opaque} s_loop_higher_inv(a: n_sized, hcount: pow2_t, j: nat, bi: nat)
+        predicate {:opaque} s_loop_higher_inv(a: n_elems, hcount: pow2_t, j: nat, bi: nat)
             requires hcount.exp <= N.exp;
             requires bi <= hcount.full;
             requires loop_view_wf();
-            requires hsize == block_size(hcount);
+            requires hsize == PV.block_size(hcount);
         {
-            && var hpoints := level_points_view(a, hsize);
+            && var hpoints := PV.level_points_view(a, hsize);
             && (forall i | 0 <= i < bi ::
-                points_eval_prefix_inv(hpoints[i], higher[bit_rev_int(i, hcount)], x_value, 2*j+2, hcount))
+                PV.points_eval_prefix_inv(hpoints[i], higher[bit_rev_int(i, hcount)], x_value, 2*j+2, hcount))
             && (forall i | bi <= i < hcount.full ::
-                points_eval_prefix_inv(hpoints[i], higher[bit_rev_int(i, hcount)], x_value, 2*j, hcount))
+                PV.points_eval_prefix_inv(hpoints[i], higher[bit_rev_int(i, hcount)], x_value, 2*j, hcount))
         }
 
-        predicate {:opaque} s_loop_lower_inv(a: n_sized, hcount: pow2_t, j: nat, bi: nat)
+        predicate {:opaque} s_loop_lower_inv(a: n_elems, hcount: pow2_t, j: nat, bi: nat)
             requires hcount.exp <= N.exp;
             requires bi <= hcount.full;
             requires loop_view_wf();
-            requires hsize == block_size(hcount);
+            requires hsize == PV.block_size(hcount);
         {
             size_count_lemma();
             && var lcount := lcount();
-            && var lpoints := level_points_view(a, lsize());
+            && var lpoints := PV.level_points_view(a, lsize());
             && (forall i | (0 <= i < bi || hcount.full <= i < bi + hcount.full) ::
-                && (points_eval_suffix_inv(lpoints[i], lower[bit_rev_int(i, lcount)], x_value, j+1, lcount)))
+                && (PV.points_eval_suffix_inv(lpoints[i], lower[bit_rev_int(i, lcount)], x_value, j+1, lcount)))
             && (forall i | (bi <= i < hcount.full || bi + hcount.full <= i < lcount.full) ::
-                points_eval_suffix_inv(lpoints[i], lower[bit_rev_int(i, lcount)], x_value, j, lcount))
+                PV.points_eval_suffix_inv(lpoints[i], lower[bit_rev_int(i, lcount)], x_value, j, lcount))
         }
 
-        predicate s_loop_inv(a: n_sized, hcount: pow2_t, j: nat, bi: nat)
+        predicate s_loop_inv(a: n_elems, hcount: pow2_t, j: nat, bi: nat)
         {
             && loop_view_wf()
             && hcount.exp <= N.exp
             && bi <= hcount.full
             && j < lsize().full
-            && hsize == block_size(hcount)
+            && hsize == PV.block_size(hcount)
             && s_loop_higher_inv(a, hcount, j, bi)
             && s_loop_lower_inv(a, hcount, j, bi)
         }
 
-        // lemma s_loop_index_bound(a: n_sized, hcount: pow2_t, j: nat, bi: nat)
+        // lemma s_loop_index_bound(a: n_elems, hcount: pow2_t, j: nat, bi: nat)
         //     requires loop_view_wf();
         //     requires hcount.exp <= N.exp;
         //     requires bi < hcount.full;
         //     requires j < lsize().full;
-        //     requires hsize == block_size(hcount);
+        //     requires hsize == PV.block_size(hcount);
         //     ensures bi + (2*j) * hcount.full + hcount.full < N.full;
         //     ensures bi + hcount.full < lcount().full;
         // {
         //     size_count_lemma();
-        //     point_view_index_bound_lemma(bi, 2 * j+1, hsize);
+        //     PV.point_view_index_bound_lemma(bi, 2 * j+1, hsize);
         //     LemmaMulIsDistributive(hcount.full, 2*j, 1);
         //     assert (2*j) * hcount.full + hcount.full == (2*j + 1) * hcount.full;
         // }
 
-        lemma higher_points_view_index_lemma(a: n_sized, hcount: pow2_t, j: nat, bi: nat)
+        lemma higher_points_view_index_lemma(a: n_elems, hcount: pow2_t, j: nat, bi: nat)
             returns (s: nat)
     
             requires s_loop_inv(a, hcount, j, bi);
             requires bi < hcount.full
             ensures s == bi + (2*j) * hcount.full;
             ensures s + hcount.full < N.full;
-            ensures a[s] == level_points_view(a, hsize)[bi][2*j];
-            ensures s == point_view_index(bi, 2*j, hsize);
-            ensures a[s+hcount.full] == level_points_view(a, hsize)[bi][2*j+1];
-            ensures s+hcount.full == point_view_index(bi, 2*j+1, hsize);
+            ensures a[s] == PV.level_points_view(a, hsize)[bi][2*j];
+            ensures s == PV.point_view_index(bi, 2*j, hsize);
+            ensures a[s+hcount.full] == PV.level_points_view(a, hsize)[bi][2*j+1];
+            ensures s+hcount.full == PV.point_view_index(bi, 2*j+1, hsize);
         {
             size_count_lemma();
-            var hpoints := level_points_view(a, hsize);
+            var hpoints := PV.level_points_view(a, hsize);
             LemmaMulNonnegative(2*j, hcount.full);
             s := bi + (2*j) * hcount.full;
 
             calc == {
                 hpoints[bi][2*j];
-                points_view(a, bi, hsize)[2*j];
-                a[point_view_index(bi, 2*j, hsize)];
+                PV.points_view(a, bi, hsize)[2*j];
+                a[PV.point_view_index(bi, 2*j, hsize)];
                 {
-                    assert s == point_view_index(bi, 2*j, hsize);
+                    assert s == PV.point_view_index(bi, 2*j, hsize);
                 }
                 a[s];
             }
 
             calc == {
                 s + hcount.full;
-                point_view_index(bi, 2*j, hsize) + hcount.full;
+                PV.point_view_index(bi, 2*j, hsize) + hcount.full;
                 bi + (2*j) * hcount.full + hcount.full;
                 {
                     LemmaMulIsDistributiveAddOtherWayAuto();
                 }
                 bi + (2*j+1) * hcount.full;
-                point_view_index(bi, 2*j+1, hsize);
+                PV.point_view_index(bi, 2*j+1, hsize);
             }
 
             calc == {
                 hpoints[bi][2*j+1];
-                points_view(a, bi, hsize)[2*j+1];
-                a[point_view_index(bi, 2*j+1, hsize)];
+                PV.points_view(a, bi, hsize)[2*j+1];
+                a[PV.point_view_index(bi, 2*j+1, hsize)];
                 a[s + hcount.full];
             }
         }
 
-        lemma lower_points_view_index_lemma(a: n_sized, hcount: pow2_t, j: nat, bi: nat)
+        lemma lower_points_view_index_lemma(a: n_elems, hcount: pow2_t, j: nat, bi: nat)
             returns (s: nat)
 
             requires s_loop_inv(a, hcount, j, bi);
@@ -303,13 +314,13 @@ abstract module ct_std2rev_model {
             ensures s == bi + (2*j) * hcount.full;
             ensures s + hcount.full < N.full;
             ensures bi + hcount.full < lcount().full;
-            ensures a[s] == level_points_view(a, lsize())[bi][j];
-            ensures s == point_view_index(bi, j, lsize());
-            ensures a[s+hcount.full] == level_points_view(a, lsize())[bi+hcount.full][j];
-            ensures s+hcount.full == point_view_index(bi+hcount.full, j, lsize());
+            ensures a[s] == PV.level_points_view(a, lsize())[bi][j];
+            ensures s == PV.point_view_index(bi, j, lsize());
+            ensures a[s+hcount.full] == PV.level_points_view(a, lsize())[bi+hcount.full][j];
+            ensures s+hcount.full == PV.point_view_index(bi+hcount.full, j, lsize());
         {
             size_count_lemma();
-            var lpoints := level_points_view(a, lsize());
+            var lpoints := PV.level_points_view(a, lsize());
             LemmaMulNonnegative(2*j, hcount.full);
             s := bi + (2*j) * hcount.full;
 
@@ -320,13 +331,13 @@ abstract module ct_std2rev_model {
                     LemmaMulProperties();
                 }
                 bi + j * (2*hcount.full);
-                point_view_index(bi, j, lsize());
+                PV.point_view_index(bi, j, lsize());
             }
 
             calc == {
                 lpoints[bi][j];
-                points_view(a, bi, lsize())[j];
-                a[point_view_index(bi, j, lsize())];
+                PV.points_view(a, bi, lsize())[j];
+                a[PV.point_view_index(bi, j, lsize())];
                 a[s];
             }
 
@@ -338,13 +349,13 @@ abstract module ct_std2rev_model {
                 }
                 bi + hcount.full + j * (2 * hcount.full);
                 bi + hcount.full + j * lcount().full;
-                point_view_index(bi +  hcount.full, j, lsize());
+                PV.point_view_index(bi +  hcount.full, j, lsize());
             }
 
             calc == {
                 lpoints[bi+hcount.full][j];
-                points_view(a, bi+hcount.full, lsize())[j];
-                a[point_view_index(bi+hcount.full, j, lsize())];
+                PV.points_view(a, bi+hcount.full, lsize())[j];
+                a[PV.point_view_index(bi+hcount.full, j, lsize())];
                 a[s+hcount.full];
             }
         }
@@ -370,60 +381,60 @@ abstract module ct_std2rev_model {
             higher[bit_rev_int(bi, hcount())]
         }
     
-        lemma lower_points_view_value_lemma(a: n_sized, hcount: pow2_t, j: nat, bi: nat, s: nat)
+        lemma lower_points_view_value_lemma(a: n_elems, hcount: pow2_t, j: nat, bi: nat, s: nat)
             requires s_loop_inv(a, hcount, j, bi);
             requires bi < hcount.full;
             requires s == bi + (2*j) * hcount.full;
             ensures s + hcount.full < N.full;
             ensures bi + hcount.full < lcount().full;
-            ensures a[s] == poly_eval(get_even_poly(bi), x_value(j, lcount()));
-            ensures a[s+hcount.full] == poly_eval(get_odd_poly(bi), x_value(j, lcount()));
+            ensures a[s] == MQP.poly_eval(get_even_poly(bi), x_value(j, lcount()));
+            ensures a[s+hcount.full] == MQP.poly_eval(get_odd_poly(bi), x_value(j, lcount()));
         {
             size_count_lemma();
             var _ := lower_points_view_index_lemma(a, hcount, j, bi);
-            var lpoints := level_points_view(a, lsize());
+            var lpoints := PV.level_points_view(a, lsize());
             var lcount := lcount();
 
             var e_poly := get_even_poly(bi);
             var e_points := lpoints[bi];
 
-            assert a[s] == poly_eval(e_poly, x_value(j, lcount)) by {
-                assert points_eval_suffix_inv(e_points, e_poly, x_value, j, lcount) by {
+            assert a[s] == MQP.poly_eval(e_poly, x_value(j, lcount)) by {
+                assert PV.points_eval_suffix_inv(e_points, e_poly, x_value, j, lcount) by {
                     reveal s_loop_lower_inv();
                 }
-                reveal points_eval_suffix_inv();
+                reveal PV.points_eval_suffix_inv();
                 assert a[s] == e_points[j];
             }
 
             var o_poly := get_odd_poly(bi);
             var o_points := lpoints[bi+hcount.full];
 
-            assert a[s+hcount.full] == poly_eval(o_poly, x_value(j, lcount)) by {
-                assert points_eval_suffix_inv(o_points, o_poly, x_value, j, lcount) by {
+            assert a[s+hcount.full] == MQP.poly_eval(o_poly, x_value(j, lcount)) by {
+                assert PV.points_eval_suffix_inv(o_points, o_poly, x_value, j, lcount) by {
                     reveal s_loop_lower_inv();
                 }
-                reveal points_eval_suffix_inv();
+                reveal PV.points_eval_suffix_inv();
                 assert a[s+hcount.full] == lpoints[bi+hcount.full][j];
             }
         }
 
-        lemma level_polys_bitrev_index_correspondence_lemma(a: n_sized, hcount: pow2_t, j: nat, bi: nat)
+        lemma level_polys_bitrev_index_correspondence_lemma(a: n_elems, hcount: pow2_t, j: nat, bi: nat)
             requires s_loop_inv(a, hcount, j, bi);
             requires bi < hcount.full
             ensures |get_full_poly(bi)| == hsize.full;
             ensures bi + hcount.full < lcount().full;
-            ensures get_even_poly(bi) == even_indexed_items(get_full_poly(bi), hsize);
-            ensures get_odd_poly(bi) == odd_indexed_items(get_full_poly(bi), hsize);
+            ensures get_even_poly(bi) == MQP.even_indexed_items(get_full_poly(bi), hsize);
+            ensures get_odd_poly(bi) == MQP.odd_indexed_items(get_full_poly(bi), hsize);
         {
             size_count_lemma();
 
             var ri := bit_rev_int(bi, hcount);
             var poly := higher[ri];
 
-            level_polys_index_correspondence_lemma(coefficients, higher, hsize, ri, lower);
+            PV.level_polys_index_correspondence_lemma(coefficients, higher, hsize, ri, lower);
 
-            assert even_indexed_items(poly, hsize) == lower[2 * ri];
-            assert odd_indexed_items(poly, hsize) == lower[2 * ri + 1];
+            assert MQP.even_indexed_items(poly, hsize) == lower[2 * ri];
+            assert MQP.odd_indexed_items(poly, hsize) == lower[2 * ri + 1];
 
             bit_rev_int_lemma0(bi, hcount);
             bit_rev_int_lemma1(bi, hcount);
@@ -431,23 +442,23 @@ abstract module ct_std2rev_model {
             // assert bit_rev_int(bi + hcount.full, lcount()) == 2 * ri + 1;
         }
 
-        predicate s_loop_update(a: n_sized, a': n_sized, hcount: pow2_t, j: nat, bi: nat)
+        predicate s_loop_update(a: n_elems, a': n_elems, hcount: pow2_t, j: nat, bi: nat)
             requires s_loop_inv(a, hcount, j, bi);
             requires x_value.requires(2*j, hcount);
             requires bi < hcount.full
         {
             var s := bi + (2*j) * hcount.full;
-            var w := mqmul(x_value(2 * j, hcount), R);
-            point_view_index_bound_lemma(bi, 2 * j+1, hsize);
-            point_view_index_bound_lemma(bi, 2 * j, hsize);
+            var w := MQP.mqmul(x_value(2 * j, hcount), R);
+            PV.point_view_index_bound_lemma(bi, 2 * j+1, hsize);
+            PV.point_view_index_bound_lemma(bi, 2 * j, hsize);
             LemmaMulIsDistributive(hcount.full, 2*j, 1);
             assert (2*j) * hcount.full + hcount.full == (2*j + 1) * hcount.full;
             var s' := s+hcount.full; 
-            a' == a[s := mqadd(a[s], montmul(a[s'], w))]
-                [s' := mqsub(a[s], montmul(a[s'], w))]
+            a' == a[s := MQP.mqadd(a[s], MQP.montmul(a[s'], w))]
+                [s' := MQP.mqsub(a[s], MQP.montmul(a[s'], w))]
         }
 
-        lemma s_loop_perserves_higher_inv_lemma(a: n_sized, a': n_sized, hcount: pow2_t, j: nat, bi: nat)
+        lemma s_loop_perserves_higher_inv_lemma(a: n_elems, a': n_elems, hcount: pow2_t, j: nat, bi: nat)
             requires s_loop_inv(a, hcount, j, bi);
             requires x_value.requires(2*j, hcount);
             requires bi < hcount.full
@@ -458,31 +469,31 @@ abstract module ct_std2rev_model {
 
             var s := higher_points_view_index_lemma(a, hcount, j, bi);
             var s' := s+hcount.full;
-            assert s == point_view_index(bi, 2*j, hsize);
-            assert s' == point_view_index(bi, 2*j + 1, hsize);
+            assert s == PV.point_view_index(bi, 2*j, hsize);
+            assert s' == PV.point_view_index(bi, 2*j + 1, hsize);
 
-            // var vo := mqadd(a[s], mqmul(a[s'], w));
-            // var ve := mqsub(a[s], mqmul(a[s'], w));
+            // var vo := MQP.mqadd(a[s], MQP.mqmul(a[s'], w));
+            // var ve := mqsub(a[s], MQP.mqmul(a[s'], w));
 
-            var hpoints := level_points_view(a, hsize);
-            var hpoints' := level_points_view(a', hsize);
+            var hpoints := PV.level_points_view(a, hsize);
+            var hpoints' := PV.level_points_view(a', hsize);
             var size := hsize.full;
 
             forall i | (0 <= i < bi || bi + 1 <= i < hcount.full)
                 ensures hpoints[i] == hpoints'[i];
-                ensures 0 <= i < bi ==> points_eval_prefix_inv(hpoints'[i], higher[bit_rev_int(i, hcount)], x_value, 2*j+2, hcount);
-                ensures bi + 1 <= i < hcount.full ==> points_eval_prefix_inv(hpoints'[i], higher[bit_rev_int(i, hcount)], x_value, 2*j, hcount);
+                ensures 0 <= i < bi ==> PV.points_eval_prefix_inv(hpoints'[i], higher[bit_rev_int(i, hcount)], x_value, 2*j+2, hcount);
+                ensures bi + 1 <= i < hcount.full ==> PV.points_eval_prefix_inv(hpoints'[i], higher[bit_rev_int(i, hcount)], x_value, 2*j, hcount);
             {
                 var left := hpoints[i];
                 var right := hpoints'[i];
     
                 assert left == right by {
                     forall k | 0 <= k < hsize.full 
-                        ensures a[point_view_index(i, k, hsize)]
-                            == a'[point_view_index(i, k, hsize)];
+                        ensures a[PV.point_view_index(i, k, hsize)]
+                            == a'[PV.point_view_index(i, k, hsize)];
                     {
-                        point_view_index_disjont_lemma(i, k, bi, 2*j, hsize);
-                        point_view_index_disjont_lemma(i, k, bi, 2*j+1, hsize);
+                        PV.point_view_index_disjont_lemma(i, k, bi, 2*j, hsize);
+                        PV.point_view_index_disjont_lemma(i, k, bi, 2*j+1, hsize);
                     }
                 }
             }
@@ -491,17 +502,17 @@ abstract module ct_std2rev_model {
             var right := hpoints'[bi];
             var poly := higher[bit_rev_int(bi, hcount)];
 
-            assert points_eval_prefix_inv(right, poly, x_value, 2*j+2, hcount) by {
-                reveal points_eval_prefix_inv();
+            assert PV.points_eval_prefix_inv(right, poly, x_value, 2*j+2, hcount) by {
+                reveal PV.points_eval_prefix_inv();
                 forall k | 0 <= k < 2*j+2 
-                    ensures poly_eval(poly, x_value(k, hcount)) == right[k];
+                    ensures MQP.poly_eval(poly, x_value(k, hcount)) == right[k];
                 {
                     if k != 2*j && k != 2*j+1 {
-                        point_view_index_disjont_lemma(bi, k, bi, 2*j, hsize);
-                        point_view_index_disjont_lemma(bi, k, bi, 2*j+1, hsize);
+                        PV.point_view_index_disjont_lemma(bi, k, bi, 2*j, hsize);
+                        PV.point_view_index_disjont_lemma(bi, k, bi, 2*j+1, hsize);
                         assert right[k] == left[k];
                     } else {
-                        var w := mqmul(x_value(2 * j, hcount), R);
+                        var w := MQP.mqmul(x_value(2 * j, hcount), R);
                         ct_butterfly_even_lemma(this, a, hcount, j, bi, s, w);
                         ct_butterfly_odd_lemma(this, a, hcount, j, bi, s, w);
                     }
@@ -509,7 +520,7 @@ abstract module ct_std2rev_model {
             }
         }
 
-        lemma s_loop_perserves_lower_inv_lemma(a: n_sized, a': n_sized, hcount: pow2_t, j: nat, bi: nat)
+        lemma s_loop_perserves_lower_inv_lemma(a: n_elems, a': n_elems, hcount: pow2_t, j: nat, bi: nat)
             requires s_loop_inv(a, hcount, j, bi);
             requires bi < hcount.full
             requires s_loop_update(a, a', hcount, j, bi);
@@ -518,54 +529,54 @@ abstract module ct_std2rev_model {
             size_count_lemma();
             var s := lower_points_view_index_lemma(a, hcount, j, bi);
             var s' := s+hcount.full;
-            assert s == point_view_index(bi, j, lsize());
-            assert s+hcount.full == point_view_index(bi+hcount.full, j, lsize());
+            assert s == PV.point_view_index(bi, j, lsize());
+            assert s+hcount.full == PV.point_view_index(bi+hcount.full, j, lsize());
 
             reveal s_loop_lower_inv();
 
-            var lpoints := level_points_view(a, lsize());
-            var lpoints' := level_points_view(a', lsize());
+            var lpoints := PV.level_points_view(a, lsize());
+            var lpoints' := PV.level_points_view(a', lsize());
             var lsize := lsize();
             var count := lcount();
 
             forall i | (bi + 1 <= i < hcount.full || bi + hcount.full + 1 <= i < count.full) 
-                ensures points_eval_suffix_inv(lpoints'[i], lower[bit_rev_int(i, count)], x_value, j, count);
+                ensures PV.points_eval_suffix_inv(lpoints'[i], lower[bit_rev_int(i, count)], x_value, j, count);
             {
                 var left := lpoints[i];
                 var right := lpoints'[i];
     
                 assert left == right by {
                     forall k | 0 <= k < lsize.full 
-                        ensures a[point_view_index(i, k, lsize)]
-                            == a'[point_view_index(i, k, lsize)];
+                        ensures a[PV.point_view_index(i, k, lsize)]
+                            == a'[PV.point_view_index(i, k, lsize)];
                     {
-                        point_view_index_disjont_lemma(i, k, bi, j, lsize);
-                        point_view_index_disjont_lemma(i, k, bi + hcount.full, j, lsize);
+                        PV.point_view_index_disjont_lemma(i, k, bi, j, lsize);
+                        PV.point_view_index_disjont_lemma(i, k, bi + hcount.full, j, lsize);
                     }
                 }
             }
         
             forall i | (0 <= i <= bi || hcount.full <= i <= bi + hcount.full)
-                ensures points_eval_suffix_inv(lpoints'[i], lower[bit_rev_int(i, count)], x_value, j+1, count);
+                ensures PV.points_eval_suffix_inv(lpoints'[i], lower[bit_rev_int(i, count)], x_value, j+1, count);
             {
                 var left := lpoints[i];
                 var right := lpoints'[i];
                 var poly := lower[bit_rev_int(i, count)];
 
                 if i == bi || i == bi + hcount.full {
-                    assert points_eval_suffix_inv(right, poly, x_value, j+1, count) by {
-                        reveal points_eval_suffix_inv();
+                    assert PV.points_eval_suffix_inv(right, poly, x_value, j+1, count) by {
+                        reveal PV.points_eval_suffix_inv();
                         forall k | j + 1 <= k < lsize.full
                             ensures right[k] == left[k];
-                            ensures poly_eval(poly, x_value(k, count)) == right[k];
+                            ensures MQP.poly_eval(poly, x_value(k, count)) == right[k];
                         {
-                            // assert left[k] == a[point_view_index(bi, k, lsize)];
-                            // assert right[k] == a'[point_view_index(bi, k, lsize)];
+                            // assert left[k] == a[PV.point_view_index(bi, k, lsize)];
+                            // assert right[k] == a'[PV.point_view_index(bi, k, lsize)];
 
-                            point_view_index_disjont_lemma(bi, k, bi, j, lsize);
-                            point_view_index_disjont_lemma(bi, k, bi + hcount.full, j, lsize);
-                            point_view_index_disjont_lemma(bi + hcount.full, k, bi, j, lsize);
-                            point_view_index_disjont_lemma(bi + hcount.full, k, bi + hcount.full, j, lsize);
+                            PV.point_view_index_disjont_lemma(bi, k, bi, j, lsize);
+                            PV.point_view_index_disjont_lemma(bi, k, bi + hcount.full, j, lsize);
+                            PV.point_view_index_disjont_lemma(bi + hcount.full, k, bi, j, lsize);
+                            PV.point_view_index_disjont_lemma(bi + hcount.full, k, bi + hcount.full, j, lsize);
 
                             assert right[k] == left[k];
                         }
@@ -573,18 +584,18 @@ abstract module ct_std2rev_model {
                 } else {
                     assert left == right by {
                         forall k | 0 <= k < lsize.full 
-                            ensures a[point_view_index(i, k, lsize)]
-                                == a'[point_view_index(i, k, lsize)];
+                            ensures a[PV.point_view_index(i, k, lsize)]
+                                == a'[PV.point_view_index(i, k, lsize)];
                         {
-                            point_view_index_disjont_lemma(i, k, bi, j, lsize);
-                            point_view_index_disjont_lemma(i, k, bi + hcount.full, j, lsize);
+                            PV.point_view_index_disjont_lemma(i, k, bi, j, lsize);
+                            PV.point_view_index_disjont_lemma(i, k, bi + hcount.full, j, lsize);
                         }
                     }
                 }
             }
         }
 
-        lemma s_loop_inv_peri_lemma(a: n_sized, a': n_sized, hcount: pow2_t, j: nat, bi: nat)
+        lemma s_loop_inv_peri_lemma(a: n_elems, a': n_elems, hcount: pow2_t, j: nat, bi: nat)
             requires s_loop_inv(a, hcount, j, bi);
             requires bi < hcount.full
             requires s_loop_update(a, a', hcount, j, bi);
@@ -594,7 +605,7 @@ abstract module ct_std2rev_model {
             s_loop_perserves_lower_inv_lemma(a, a', hcount, j, bi);
         }
 
-        lemma s_loop_inv_pre_lemma(a: n_sized, hcount: pow2_t, j: nat)
+        lemma s_loop_inv_pre_lemma(a: n_elems, hcount: pow2_t, j: nat)
             requires j_loop_inv(a, hcount, j);
             requires j < lsize().full;
             ensures s_loop_inv(a, hcount, j, 0);
@@ -611,10 +622,10 @@ abstract module ct_std2rev_model {
                 reveal j_loop_lower_inv();
 
                 var lcount := lcount();
-                var lpoints := level_points_view(a, lsize());
+                var lpoints := PV.level_points_view(a, lsize());
 
                 forall i | (0 <= i < hcount.full || hcount.full <= i < lcount.full)
-                    ensures points_eval_suffix_inv(lpoints[i], lower[bit_rev_int(i, lcount)], x_value, j, lcount);
+                    ensures PV.points_eval_suffix_inv(lpoints[i], lower[bit_rev_int(i, lcount)], x_value, j, lcount);
                 {
                     assert (0 <= i < hcount.full || hcount.full <= i < lcount.full)
                         ==> (0 <= i < lcount.full);
@@ -622,16 +633,16 @@ abstract module ct_std2rev_model {
             }
         }
 
-        lemma s_loop_inv_post_lemma(a: n_sized, hcount: pow2_t, j: nat, bi: nat)
+        lemma s_loop_inv_post_lemma(a: n_elems, hcount: pow2_t, j: nat, bi: nat)
             requires s_loop_inv(a, hcount, j, bi);
             requires bi == hcount.full;
             ensures j_loop_inv(a, hcount, j + 1)
         {
             assert j_loop_higher_inv(a, hcount, j+1) by {
-                var hpoints := level_points_view(a, hsize);
+                var hpoints := PV.level_points_view(a, hsize);
                 reveal s_loop_higher_inv();
                 forall i | 0 <= i < |hpoints|
-                    ensures points_eval_prefix_inv(hpoints[i], higher[bit_rev_int(i, hcount)], x_value, 2*j+2, hcount);
+                    ensures PV.points_eval_prefix_inv(hpoints[i], higher[bit_rev_int(i, hcount)], x_value, 2*j+2, hcount);
                 {
                 }
                 reveal j_loop_higher_inv();
@@ -641,31 +652,31 @@ abstract module ct_std2rev_model {
 
             assert j_loop_lower_inv(a, hcount, j+1) by {
                 var lcount := lcount();
-                var lpoints := level_points_view(a, lsize());
+                var lpoints := PV.level_points_view(a, lsize());
                 reveal s_loop_lower_inv();
                 forall i | 0 <= i < |lpoints|
-                    ensures points_eval_suffix_inv(lpoints[i], lower[bit_rev_int(i, lcount)], x_value, j+1, lcount);
+                    ensures PV.points_eval_suffix_inv(lpoints[i], lower[bit_rev_int(i, lcount)], x_value, j+1, lcount);
                 {
                 }
                 reveal j_loop_lower_inv();
             }
         }
 
-        lemma j_loop_inv_pre_lemma(a: n_sized, hcount: pow2_t)
+        lemma j_loop_inv_pre_lemma(a: n_elems, hcount: pow2_t)
             requires 0 <= hcount.exp < N.exp;
             requires t_loop_inv(a, pow2_double(hcount), coefficients);
             requires loop_view_wf();
-            requires hsize == block_size(hcount);
+            requires hsize == PV.block_size(hcount);
             ensures j_loop_inv(a, hcount, 0);
         {
             assert j_loop_higher_inv(a, hcount, 0) by {
-                var hpoints := level_points_view(a, hsize);
+                var hpoints := PV.level_points_view(a, hsize);
                 forall i | 0 <= i < hcount.full
-                    ensures points_eval_prefix_inv(hpoints[i], higher[bit_rev_int(i, hcount)], x_value, 0, hcount);
+                    ensures PV.points_eval_prefix_inv(hpoints[i], higher[bit_rev_int(i, hcount)], x_value, 0, hcount);
                 {
-                    unifromly_sized_instance_lemma(hpoints, hsize, i);
-                    unifromly_sized_instance_lemma(higher, hsize, bit_rev_int(i, hcount));
-                    points_eval_prefix_inv_vacuous_lemma(hpoints[i], higher[bit_rev_int(i, hcount)], x_value, hcount);
+                    PV.unifromly_sized_instance_lemma(hpoints, hsize, i);
+                    PV.unifromly_sized_instance_lemma(higher, hsize, bit_rev_int(i, hcount));
+                    PV.points_eval_prefix_inv_vacuous_lemma(hpoints[i], higher[bit_rev_int(i, hcount)], x_value, hcount);
                 }
                 reveal j_loop_higher_inv();
             }
@@ -675,32 +686,32 @@ abstract module ct_std2rev_model {
             assert j_loop_lower_inv(a, hcount, 0) by {
                 reveal t_loop_inv();
                 var lcount := lcount();
-                var lpoints := level_points_view(a, lsize());
+                var lpoints := PV.level_points_view(a, lsize());
                 forall i | 0 <= i < lcount.full
-                    ensures points_eval_suffix_inv(lpoints[i], lower[bit_rev_int(i, lcount)], x_value, 0, lcount)
+                    ensures PV.points_eval_suffix_inv(lpoints[i], lower[bit_rev_int(i, lcount)], x_value, 0, lcount)
                 {
-                    reveal points_eval_suffix_inv();
+                    reveal PV.points_eval_suffix_inv();
                 }
                 reveal j_loop_lower_inv();
             }
         }
 
-        lemma j_loop_inv_post_lemma(a: n_sized, hcount: pow2_t, j: nat)
+        lemma j_loop_inv_post_lemma(a: n_elems, hcount: pow2_t, j: nat)
             requires j_loop_inv(a, hcount, j);
             requires j == lsize().full;
             requires 0 <= hsize.exp <= N.exp;
-            requires hsize == block_size(hcount);
+            requires hsize == PV.block_size(hcount);
             ensures t_loop_inv(a, hcount, coefficients);
         {
             reveal j_loop_higher_inv();
             size_count_lemma();
-            var hpoints := level_points_view(a, hsize);
+            var hpoints := PV.level_points_view(a, hsize);
 
             forall i | 0 <= i < hcount.full
-                ensures points_eval_inv(hpoints[i], higher[bit_rev_int(i, hcount)], x_value, hcount);
+                ensures PV.points_eval_inv(hpoints[i], higher[bit_rev_int(i, hcount)], x_value, hcount);
             {
-                reveal points_eval_suffix_inv();
-                reveal points_eval_prefix_inv();
+                reveal PV.points_eval_suffix_inv();
+                reveal PV.points_eval_prefix_inv();
             }
 
             assert t_loop_inv(a, hcount, coefficients) by {
@@ -709,15 +720,15 @@ abstract module ct_std2rev_model {
         }
     }
 
-    function build_loop_view(coefficients: n_sized, hcount: pow2_t): (view: loop_view)
+    function build_loop_view(coefficients: n_elems, hcount: pow2_t): (view: loop_view)
         requires 0 <= hcount.exp < N.exp
         ensures view.loop_view_wf();
     {
-        var hsize := block_size(hcount);
+        var hsize := PV.block_size(hcount);
         loop_view(
             coefficients,
-            level_polys(coefficients, pow2_half(hsize)),
-            level_polys(coefficients, hsize),
+            PV.level_polys(coefficients, pow2_half(hsize)),
+            PV.level_polys(coefficients, hsize),
             hsize)
     }
 
@@ -725,44 +736,49 @@ abstract module ct_std2rev_model {
         requires view.loop_view_wf();
         requires 2 * j < view.hsize.full;
         requires x == x_value(2 * j + 1, view.hcount());
-        ensures mqmul(x, x) == x_value(j, view.lcount());
+        ensures MQP.mqmul(x, x) == x_value(j, view.lcount());
 
     lemma x_value_even_square_lemma(view: loop_view, j: nat, x: elem)
         requires view.loop_view_wf();
         requires 2 * j < view.hsize.full;
         requires x == x_value(2 * j, view.hcount());
-        ensures mqmul(x, x) == x_value(j, view.lcount());
+        ensures MQP.mqmul(x, x) == x_value(j, view.lcount());
 
-    lemma ct_butterfly_even_lemma(view: loop_view, a: n_sized, hcount: pow2_t, j: nat, bi: nat, s: nat, w: elem)
+    lemma ct_butterfly_even_lemma(view: loop_view, a: n_elems, hcount: pow2_t, j: nat, bi: nat, s: nat, w: elem)
         requires view.s_loop_inv(a, hcount, j, bi);
         requires s == bi + (2*j) * hcount.full;
         requires bi < hcount.full
-        requires w == mqmul(x_value(2 * j, hcount), R);
+        requires w == MQP.mqmul(x_value(2 * j, hcount), R);
         ensures s + hcount.full < N.full;
         ensures bi + hcount.full < view.lcount().full;
-        ensures poly_eval(view.get_full_poly(bi), x_value(2*j, hcount))
-            == mqadd(a[s], montmul(a[s+hcount.full], w));
+        ensures MQP.poly_eval(view.get_full_poly(bi), x_value(2*j, hcount))
+            == MQP.mqadd(a[s], MQP.montmul(a[s+hcount.full], w));
 
-    lemma ct_butterfly_odd_lemma(view: loop_view, a: n_sized, hcount: pow2_t, j: nat, bi: nat, s: nat, w: elem)
+    lemma ct_butterfly_odd_lemma(view: loop_view, a: n_elems, hcount: pow2_t, j: nat, bi: nat, s: nat, w: elem)
         requires view.s_loop_inv(a, hcount, j, bi);
         requires bi < hcount.full
         requires s == bi + (2*j) * hcount.full;
-        requires w == mqmul(x_value(2 * j, hcount), R);
+        requires w == MQP.mqmul(x_value(2 * j, hcount), R);
         ensures s + hcount.full < N.full;
         ensures bi + hcount.full < view.lcount().full;
-        ensures poly_eval(view.get_full_poly(bi), x_value(2*j+1, hcount))
-            == mqsub(a[s], montmul(a[s+hcount.full], w));
+        ensures MQP.poly_eval(view.get_full_poly(bi), x_value(2*j+1, hcount))
+            == MQP.mqsub(a[s], MQP.montmul(a[s+hcount.full], w));
 }
 
-module forward_ntt refines ct_std2rev_model {
+module mq_fntt_i(CMQ: ntt_param_s) refines mq_ntt_i(CMQ) {
 
-    ghost const x_value := rev_mixed_powers_mont_x_value;
+    // function rev_mixed_powers_mont_x_value(i: nat, d: pow2_t): (r: elem)
+
+	function x_value(i: nat, d: pow2_t): (r: elem)
+    {
+        TWD.rev_mixed_powers_mont_x_value(i, d)
+    }
 
     lemma x_value_even_square_lemma(view: loop_view, j: nat, x: elem)
         // requires loop_view_wf();
         // requires 2 * j < view.hsize.full;
         // requires x == x_value(2 * j, view.hcount());
-        // ensures mqmul(x, x) == x_value(j, view.lcount());
+        // ensures MQP.mqmul(x, x) == x_value(j, view.lcount());
     {
         view.size_count_lemma();
         var hc := view.hcount();
@@ -804,7 +820,7 @@ module forward_ntt refines ct_std2rev_model {
         var temp := Pow(PSI, exp);
 
         calc == {
-            mqmul(x, x);
+            MQP.mqmul(x, x);
             ((temp % Q) * (temp % Q)) % Q;
             {
                 LemmaMulModNoopGeneral(temp, temp, Q);
@@ -823,7 +839,7 @@ module forward_ntt refines ct_std2rev_model {
         // requires 2 * j < view.hsize.full;
         // requires x_value.requires(2 * j + 1, view.hcount());
         // requires x == x_value(2 * j + 1, view.hcount());
-        // ensures mqmul(x, x) == x_value(j, view.lcount());
+        // ensures MQP.mqmul(x, x) == x_value(j, view.lcount());
     {
         view.size_count_lemma();
         var hc := view.hcount();
@@ -887,7 +903,7 @@ module forward_ntt refines ct_std2rev_model {
         }
 
         calc == {
-            mqmul(x, x);
+            MQP.mqmul(x, x);
             ((temp % Q) * (temp % Q)) % Q;
             {
                 LemmaMulModNoopGeneral(temp, temp, Q);
@@ -900,34 +916,34 @@ module forward_ntt refines ct_std2rev_model {
             Pow(PSI, 2 * bit_rev_int(j, lsize) * lcount.full + 2 * N.full + lcount.full) % Q;
             {
                 LemmaMulNonnegative(2 * bit_rev_int(j, lsize), lcount.full);
-                full_rotation_lemma(2 * bit_rev_int(j, lsize) * lcount.full + lcount.full);
+                TWD.full_rotation_lemma(2 * bit_rev_int(j, lsize) * lcount.full + lcount.full);
             }
             Pow(PSI, 2 * bit_rev_int(j, lsize) * lcount.full + lcount.full) % Q;
         }
     }
 
-    lemma ct_butterfly_even_lemma(view: loop_view, a: n_sized, hcount: pow2_t, j: nat, bi: nat, s: nat, w: elem)
+    lemma ct_butterfly_even_lemma(view: loop_view, a: n_elems, hcount: pow2_t, j: nat, bi: nat, s: nat, w: elem)
         // requires view.s_loop_inv(a, hcount, j, bi);
         // requires s == bi + (2*j) * hcount.full;
         // requires bi < hcount.full
-        // requires w == mqmul(x_value(2 * j, hcount), R);
+        // requires w == MQP.mqmul(x_value(2 * j, hcount), R);
         // ensures s + hcount.full < N.full;
         // ensures bi + hcount.full < view.lcount().full;
-        // ensures poly_eval(view.get_full_poly(bi), x_value(2*j, hcount))
-        //     == mqadd(a[s], montmul(a[s+hcount.full], w));
+        // ensures MQP.poly_eval(view.get_full_poly(bi), x_value(2*j, hcount))
+        //     == MQP.mqadd(a[s], montmul(a[s+hcount.full], w));
     {
         view.size_count_lemma();
         view.lower_points_view_value_lemma(a, hcount, j, bi, s);
         var e := a[s];
         var o := a[s+hcount.full];
-        var p := montmul(o, w);
+        var p := MQP.montmul(o, w);
 
         gbassert IsModEquivalent(p, o * x_value(2 * j, hcount), Q) by {
             assert IsModEquivalent(p, o * w * R_INV, Q) by {
                 LemmaSmallMod(p, Q);
             }
             assert IsModEquivalent(R_INV * R, 1, Q) by {
-                Nth_root_lemma();
+                CMQ.Nth_root_lemma();
             }
             assert IsModEquivalent(w, x_value(2 * j, hcount) * R, Q) by {
                 LemmaSmallMod(w, Q);
@@ -938,8 +954,8 @@ module forward_ntt refines ct_std2rev_model {
             LemmaSmallMod(p, Q);
         }
 
-        var sum := mqadd(e, p);
-        var diff := mqsub(e, p);
+        var sum := MQP.mqadd(e, p);
+        var diff := MQP.mqsub(e, p);
 
         var e_poly := view.get_even_poly(bi);
         var o_poly := view.get_odd_poly(bi);
@@ -950,30 +966,29 @@ module forward_ntt refines ct_std2rev_model {
         var x := x_value(2*j, hcount);
         var sqr := x_value(j, view.lcount());
 
-        assert e == poly_eval(e_poly, sqr);
-        assert o == poly_eval(o_poly, sqr);
+        assert e == MQP.poly_eval(e_poly, sqr);
+        assert o == MQP.poly_eval(o_poly, sqr);
 
         x_value_even_square_lemma(view, j, x);
 
-        poly_eval_split_lemma(f_poly, e_poly, o_poly, view.hsize, x);
+        MQP.poly_eval_split_lemma(f_poly, e_poly, o_poly, view.hsize, x);
     }
 
-
-    lemma ct_butterfly_odd_lemma(view: loop_view, a: n_sized, hcount: pow2_t, j: nat, bi: nat, s: nat, w: elem)
+    lemma ct_butterfly_odd_lemma(view: loop_view, a: n_elems, hcount: pow2_t, j: nat, bi: nat, s: nat, w: elem)
         // requires view.s_loop_inv(a, hcount, j, bi);
         // requires bi < hcount.full
         // requires s == bi + (2*j) * hcount.full;
-        // requires w == mqmul(x_value(2 * j, hcount), R);
+        // requires w == MQP.mqmul(x_value(2 * j, hcount), R);
         // ensures s + hcount.full < N.full;
         // ensures bi + hcount.full < view.lcount().full;
-        // ensures poly_eval(view.get_full_poly(bi), x_value(2*j+1, hcount))
+        // ensures MQP.poly_eval(view.get_full_poly(bi), x_value(2*j+1, hcount))
         //     == mqsub(a[s], montmul(a[s+hcount.full], w));
     {
         view.size_count_lemma();
         view.lower_points_view_value_lemma(a, hcount, j, bi, s);
         var e := a[s];
         var o := a[s+hcount.full];
-        var p := montmul(o, w);
+        var p := MQP.montmul(o, w);
 
         var hsize := view.hsize;
         var lsize := view.lsize();
@@ -984,7 +999,7 @@ module forward_ntt refines ct_std2rev_model {
                 LemmaSmallMod(p, Q);
             }
             assert IsModEquivalent(R_INV * R, 1, Q) by {
-                Nth_root_lemma();
+                CMQ.Nth_root_lemma();
             }
             assert IsModEquivalent(w, x_value(2*j, hcount) * R, Q) by {
                 LemmaSmallMod(w, Q);
@@ -995,7 +1010,7 @@ module forward_ntt refines ct_std2rev_model {
             LemmaSmallMod(p, Q);
         }
 
-        var diff := mqsub(e, p);
+        var diff := MQP.mqsub(e, p);
 
         var e_poly := view.get_even_poly(bi);
         var o_poly := view.get_odd_poly(bi);
@@ -1009,37 +1024,38 @@ module forward_ntt refines ct_std2rev_model {
         view.level_polys_bitrev_index_correspondence_lemma(a, hcount, j, bi);
 
         var sqr := x_value(j, lcount);
+        var rj := bit_rev_int(j, lsize);
 
         calc == {
             x_o;
             {
                 LemmaMulNonnegative(2 * bit_rev_int(2*j+1, hsize), hcount.full);
             }
-            mqpow(PSI, 2 * bit_rev_int(2*j+1, hsize) * hcount.full + hcount.full);
+            MQP.mqpow(CMQ.PSI, 2 * bit_rev_int(2*j+1, hsize) * hcount.full + hcount.full);
             {
                 bit_rev_int_lemma3(j, lsize);
-                assert bit_rev_int(2*j+1, hsize) == bit_rev_int(j, lsize) + lsize.full;
+                assert bit_rev_int(2*j+1, hsize) == rj + lsize.full;
             }
-            mqpow(PSI, 2 * (bit_rev_int(j, lsize) + lsize.full) * hcount.full + hcount.full);
+            MQP.mqpow(PSI, 2 * (rj + lsize.full) * hcount.full + hcount.full);
             {
-                gbassert 2 * (bit_rev_int(j, lsize) + lsize.full) * hcount.full == 2 * (bit_rev_int(j, lsize) * hcount.full) + N.full by {
+                gbassert 2 * (rj + lsize.full) * hcount.full == 2 * (rj * hcount.full) + N.full by {
                     assert 2 * lsize.full * hcount.full == N.full;
                 }
             }
-            mqpow(PSI, 2 * (bit_rev_int(j, lsize) * hcount.full) + N.full + hcount.full);
+            MQP.mqpow(PSI, 2 * (rj * hcount.full) + N.full + hcount.full);
             {
-                LemmaMulNonnegative(bit_rev_int(j, lsize), hcount.full);
-                half_rotation_lemma(2 * (bit_rev_int(j, lsize) * hcount.full) + hcount.full);
+                LemmaMulNonnegative(rj, hcount.full);
+                TWD.half_rotation_lemma(2 * (rj * hcount.full) + hcount.full);
             }
-            (Q - mqpow(PSI, 2 * (bit_rev_int(j, lsize) * hcount.full) + hcount.full)) % Q;
+            (Q - MQP.mqpow(PSI, 2 * (rj * hcount.full) + hcount.full)) % Q;
             {
-                LemmaMulIsAssociative(2, bit_rev_int(j, lsize), hcount.full);
+                LemmaMulIsAssociative(2, rj, hcount.full);
             }
-            (Q - mqpow(PSI, 2 * bit_rev_int(j, lsize) * hcount.full + hcount.full)) % Q;
+            (Q - MQP.mqpow(PSI, 2 * rj * hcount.full + hcount.full)) % Q;
             {
                 bit_rev_int_lemma2(j, lsize);
             }
-            (Q - mqpow(PSI, 2 * bit_rev_int(2*j, hsize) * hcount.full + hcount.full)) % Q;
+            (Q - MQP.mqpow(PSI, 2 * bit_rev_int(2*j, hsize) * hcount.full + hcount.full)) % Q;
             (Q - x_e) % Q;
             {
                 LemmaSmallMod(Q- x_e, Q);
@@ -1049,7 +1065,7 @@ module forward_ntt refines ct_std2rev_model {
 
         calc == {
             diff;
-            mqsub(e, mqmul(o, x_e));
+            MQP.mqsub(e, MQP.mqmul(o, x_e));
             {
                 LemmaMulNonnegative(o, x_e);
             }
@@ -1069,7 +1085,11 @@ module forward_ntt refines ct_std2rev_model {
             (e as int - (Q * o- x_o * o)) % Q;
             (e as int + x_o * o - Q * o) % Q;
             {
-                LemmaModMultiplesVanish(e as int + x_o * o, -(o as int), Q);
+                LemmaMulProperties();
+            }
+            (e as int + x_o * o + Q * (-o)) % Q;
+            {
+                LemmaModMultiplesVanish(-o, e as int + x_o * o, Q);
             }
             (e as int + x_o * o) % Q;
             {
@@ -1080,26 +1100,30 @@ module forward_ntt refines ct_std2rev_model {
                 LemmaSmallMod(e, Q);
             }
             (e + (x_o * o) % Q) % Q;
-            (e + mqmul(x_o, o)) % Q;
-            mqadd(e, mqmul(x_o, o));
-            mqadd(poly_eval(e_poly, sqr), mqmul(x_o, poly_eval(o_poly, sqr)));
+            (e + MQP.mqmul(x_o, o)) % Q;
+            MQP.mqadd(e, MQP.mqmul(x_o, o));
+            MQP.mqadd(MQP.poly_eval(e_poly, sqr), MQP.mqmul(x_o, MQP.poly_eval(o_poly, sqr)));
             {
-                poly_eval_split_lemma(f_poly, e_poly, o_poly, view.hsize, x_o);
+                MQP.poly_eval_split_lemma(f_poly, e_poly, o_poly, view.hsize, x_o);
             }
-            poly_eval(f_poly, x_o);
+            MQP.poly_eval(f_poly, x_o);
         }
     }
 }
 
-module inverse_ntt refines ct_std2rev_model {
+module mq_intt(CMQ: ntt_param_s) refines mq_ntt_i(CMQ) {
+    // ghost const x_value := rev_omega_inv_powers_x_value;
 
-    ghost const x_value := rev_omega_inv_powers_x_value;
+	function x_value(i: nat, d: pow2_t): (r: elem)
+    {
+        TWD.rev_omega_inv_powers_x_value(i, d)
+    }
 
     lemma x_value_even_square_lemma(view: loop_view, j: nat, x: elem)
         // requires loop_view_wf();
         // requires 2 * j < view.hsize.full;
         // requires x == x_value(2 * j, view.hcount());
-        // ensures mqmul(x, x) == x_value(j, view.lcount());
+        // ensures MQP.mqmul(x, x) == x_value(j, view.lcount());
     {
         view.size_count_lemma();
 
@@ -1112,7 +1136,7 @@ module inverse_ntt refines ct_std2rev_model {
         LemmaMulIsAssociative(2, bit_rev_int(2 * j, hsize), hc.full);
         var exp := bit_rev_int(2 * j , hsize) * hc.full;
 
-        assert x == mqpow(OMEGA_INV, exp);
+        assert x == MQP.mqpow(OMEGA_INV, exp);
 
         calc == {
             2 * exp;
@@ -1131,7 +1155,7 @@ module inverse_ntt refines ct_std2rev_model {
         var temp := Pow(OMEGA_INV, exp);
 
         calc == {
-            mqmul(x, x);
+            MQP.mqmul(x, x);
             ((temp % Q) * (temp % Q)) % Q;
             {
                 LemmaMulModNoopGeneral(temp, temp, Q);
@@ -1150,7 +1174,7 @@ module inverse_ntt refines ct_std2rev_model {
         // requires loop_view_wf();
         // requires 2 * j < hsize.full;
         // requires x == x_value(2 * j + 1, hcount());
-        // ensures mqmul(x, x) == x_value(j, lcount());
+        // ensures MQP.mqmul(x, x) == x_value(j, lcount());
     {
         view.size_count_lemma();
 
@@ -1162,7 +1186,7 @@ module inverse_ntt refines ct_std2rev_model {
         LemmaMulNonnegative(bit_rev_int(2 * j + 1, hsize), hc.full);
         LemmaMulIsAssociative(2, bit_rev_int(2 * j + 1, hsize), hc.full);
         var exp := bit_rev_int(2 * j + 1, hsize) * hc.full;   
-        assert x == mqpow(OMEGA_INV, exp);
+        assert x == MQP.mqpow(OMEGA_INV, exp);
         var temp := Pow(OMEGA_INV, exp);
 
         calc == {
@@ -1193,7 +1217,7 @@ module inverse_ntt refines ct_std2rev_model {
         }
 
         calc == {
-            mqmul(x, x);
+            MQP.mqmul(x, x);
             ((temp % Q) * (temp % Q)) % Q;
             {
                 LemmaMulModNoopGeneral(temp, temp, Q);
@@ -1206,33 +1230,33 @@ module inverse_ntt refines ct_std2rev_model {
             Pow(OMEGA_INV, bit_rev_int(j, lsize) * lcount.full + N.full) % Q;
             {
                 LemmaMulNonnegative(bit_rev_int(j, lsize), lcount.full);
-                inv_full_rotation_lemma(bit_rev_int(j, lsize) * lcount.full);
+                TWD.inv_full_rotation_lemma(bit_rev_int(j, lsize) * lcount.full);
             }
             Pow(OMEGA_INV, bit_rev_int(j, lsize) * lcount.full) % Q;
         }
     }
 
-    lemma ct_butterfly_even_lemma(view: loop_view, a: n_sized, hcount: pow2_t, j: nat, bi: nat, s: nat, w: elem)
+    lemma ct_butterfly_even_lemma(view: loop_view, a: n_elems, hcount: pow2_t, j: nat, bi: nat, s: nat, w: elem)
         // requires s_loop_inv(a, hcount, j, bi);
         // requires s == bi + (2*j) * hcount.full;
         // requires bi < hcount.full
-        // requires w == mqmul(x_value(2 * j, hcount), R);
+        // requires w == MQP.mqmul(x_value(2 * j, hcount), R);
         // ensures s + hcount.full < N.full;
         // ensures bi + hcount.full < lcount().full;
-        // ensures poly_eval(get_full_poly(bi), x_value(2*j, hcount)) == mqadd(a[s], montmul(a[s+hcount.full], w));
+        // ensures MQP.poly_eval(get_full_poly(bi), x_value(2*j, hcount)) == MQP.mqadd(a[s], montmul(a[s+hcount.full], w));
     {
         view.size_count_lemma();
         view.lower_points_view_value_lemma(a, hcount, j, bi, s);
         var e := a[s];
         var o := a[s+hcount.full];
-        var p := montmul(o, w);
+        var p := MQP.montmul(o, w);
 
         gbassert IsModEquivalent(p, o * x_value(2 * j, hcount), Q) by {
             assert IsModEquivalent(p, o * w * R_INV, Q) by {
                 LemmaSmallMod(p, Q);
             }
             assert IsModEquivalent(R_INV * R, 1, Q) by {
-                Nth_root_lemma();
+                CMQ.Nth_root_lemma();
             }
             assert IsModEquivalent(w, x_value(2 * j, hcount) * R, Q) by {
                 LemmaSmallMod(w, Q);
@@ -1243,8 +1267,8 @@ module inverse_ntt refines ct_std2rev_model {
             LemmaSmallMod(p, Q);
         }
 
-        var sum := mqadd(e, p);
-        var diff := mqsub(e, p);
+        var sum := MQP.mqadd(e, p);
+        var diff := MQP.mqsub(e, p);
 
         var e_poly := view.get_even_poly(bi);
         var o_poly := view.get_odd_poly(bi);
@@ -1255,22 +1279,22 @@ module inverse_ntt refines ct_std2rev_model {
         var x := x_value(2*j, hcount);
         var sqr := x_value(j, view.lcount());
 
-        assert e == poly_eval(e_poly, sqr);
-        assert o == poly_eval(o_poly, sqr);
+        assert e == MQP.poly_eval(e_poly, sqr);
+        assert o == MQP.poly_eval(o_poly, sqr);
 
         x_value_even_square_lemma(view, j, x);
 
-        poly_eval_split_lemma(f_poly, e_poly, o_poly, view.hsize, x);
+        MQP.poly_eval_split_lemma(f_poly, e_poly, o_poly, view.hsize, x);
     }
 
-    lemma ct_butterfly_odd_lemma(view: loop_view, a: n_sized, hcount: pow2_t, j: nat, bi: nat, s: nat, w: elem)
+    lemma ct_butterfly_odd_lemma(view: loop_view, a: n_elems, hcount: pow2_t, j: nat, bi: nat, s: nat, w: elem)
         // requires s_loop_inv(a, hcount, j, bi);
         // requires bi < hcount.full
         // requires s == bi + (2*j) * hcount.full;
-        // requires w == mqmul(x_value(2 * j, hcount), R);
+        // requires w == MQP.mqmul(x_value(2 * j, hcount), R);
         // ensures s + hcount.full < N.full;
         // ensures bi + hcount.full < lcount().full;
-        // ensures poly_eval(get_full_poly(bi), x_value(2*j+1, hcount))
+        // ensures MQP.poly_eval(get_full_poly(bi), x_value(2*j+1, hcount))
         //     == mqsub(a[s], montmul(a[s+hcount.full], w));
     {
         view.size_count_lemma();
@@ -1283,14 +1307,14 @@ module inverse_ntt refines ct_std2rev_model {
         view.lower_points_view_value_lemma(a, hcount, j, bi, s);
         var e := a[s];
         var o := a[s+hcount.full];
-        var p := montmul(o, w);
+        var p := MQP.montmul(o, w);
 
         gbassert IsModEquivalent(p, o * x_value(2*j, hcount), Q) by {
             assert IsModEquivalent(p, o * w * R_INV, Q) by {
                 LemmaSmallMod(p, Q);
             }
             assert IsModEquivalent(R_INV * R, 1, Q) by {
-                Nth_root_lemma();
+                CMQ.Nth_root_lemma();
             }
             assert IsModEquivalent(w, x_value(2*j, hcount) * R, Q) by {
                 LemmaSmallMod(w, Q);
@@ -1301,7 +1325,7 @@ module inverse_ntt refines ct_std2rev_model {
             LemmaSmallMod(p, Q);
         }
 
-        var diff := mqsub(e, p);
+        var diff :=  MQP.mqsub(e, p);
 
         var e_poly := view.get_even_poly(bi);
         var o_poly := view.get_odd_poly(bi);
@@ -1321,23 +1345,23 @@ module inverse_ntt refines ct_std2rev_model {
             {
                 LemmaMulNonnegative(bit_rev_int(2*j+1, hsize), hcount.full);
             }
-            mqpow(OMEGA_INV, bit_rev_int(2*j+1, hsize) * hcount.full);
+            MQP.mqpow(OMEGA_INV, bit_rev_int(2*j+1, hsize) * hcount.full);
             {
                 bit_rev_int_lemma3(j, lsize);
                 assert bit_rev_int(2*j+1, hsize) == bit_rev_int(j, lsize) + lsize.full;
             }
-            mqpow(OMEGA_INV, (bit_rev_int(j, lsize) + lsize.full) * hcount.full);
+            MQP.mqpow(OMEGA_INV, (bit_rev_int(j, lsize) + lsize.full) * hcount.full);
             {
                 LemmaMulIsDistributive(hcount.full, bit_rev_int(j, lsize), lsize.full);
             }
-            mqpow(OMEGA_INV, bit_rev_int(j, lsize) * hcount.full + lsize.full * hcount.full);
+            MQP.mqpow(OMEGA_INV, bit_rev_int(j, lsize) * hcount.full + lsize.full * hcount.full);
             {
                 bit_rev_int_lemma2(j, lsize);
             }
-            mqpow(OMEGA_INV, bit_rev_int(2 * j, hsize) * hcount.full + lsize.full * hcount.full);
+            MQP.mqpow(OMEGA_INV, bit_rev_int(2 * j, hsize) * hcount.full + lsize.full * hcount.full);
             {
                 LemmaMulNonnegative(bit_rev_int(2 * j, hsize), hcount.full);
-                inv_half_rotation_lemma(bit_rev_int(2 * j, hsize) * hcount.full);
+                TWD.inv_half_rotation_lemma(bit_rev_int(2 * j, hsize) * hcount.full);
                 assert lsize.full * hcount.full == N.full / 2 by {
                     LemmaMulProperties();
                 }
@@ -1351,7 +1375,7 @@ module inverse_ntt refines ct_std2rev_model {
 
         calc == {
             diff;
-            mqsub(e, mqmul(o, x_e));
+            MQP.mqsub(e, MQP.mqmul(o, x_e));
             {
                 LemmaMulNonnegative(o, x_e);
             }
@@ -1368,10 +1392,13 @@ module inverse_ntt refines ct_std2rev_model {
             {
                 LemmaMulIsDistributive(o, Q, x_o);
             }
-            (e as int - (Q * o- x_o * o)) % Q;
             (e as int + x_o * o - Q * o) % Q;
             {
-                LemmaModMultiplesVanish(e as int + x_o * o, -(o as int), Q);
+                LemmaMulProperties();
+            }
+            (e as int + x_o * o + Q * (-o)) % Q;
+            {
+                LemmaModMultiplesVanish(-o, e as int + x_o * o, Q);
             }
             (e as int + x_o * o) % Q;
             {
@@ -1382,13 +1409,13 @@ module inverse_ntt refines ct_std2rev_model {
                 LemmaSmallMod(e, Q);
             }
             (e + (x_o * o) % Q) % Q;
-            (e + mqmul(x_o, o)) % Q;
-            mqadd(e, mqmul(x_o, o));
-            mqadd(poly_eval(e_poly, sqr), mqmul(x_o, poly_eval(o_poly, sqr)));
+            (e + MQP.mqmul(x_o, o)) % Q;
+            MQP.mqadd(e, MQP.mqmul(x_o, o));
+            MQP.mqadd(MQP.poly_eval(e_poly, sqr), MQP.mqmul(x_o, MQP.poly_eval(o_poly, sqr)));
             {
-                poly_eval_split_lemma(f_poly, e_poly, o_poly, hsize, x_o);
+                MQP.poly_eval_split_lemma(f_poly, e_poly, o_poly, hsize, x_o);
             }
-            poly_eval(f_poly, x_o);
+            MQP.poly_eval(f_poly, x_o);
         }
     }
 }
