crypto_specs/mq_norm.s.dfy
@@ -1,0 +1,35 @@
+include "ntt_param.s.dfy"
+
+module mq_norm_s(MQ: ntt_param_s) {
+    const Q_HLAF := MQ.Q / 2
+
+    predicate int_is_normalized(e: int)
+    {
+        -Q_HLAF <= e <= Q_HLAF
+    }
+
+    type nelem = e: int | int_is_normalized(e)
+
+    // 0 <= e < Q -> -Q/2 <= e <= Q/2
+    function normalize(e: MQ.elem): nelem
+    {
+        if e <= Q_HLAF then e else e as int - MQ.Q
+    }
+
+    // -Q/2 <= e < Q/2 -> 0 <= e <= Q 
+    function denormalize(e: nelem): MQ.elem
+    {
+        if e >= 0 then e else e + MQ.Q
+    }
+
+    lemma normalize_inverse(e: MQ.elem)
+        ensures denormalize(normalize(e)) == e;
+    {}
+
+    lemma denormalize_inverse(e: nelem)
+        ensures normalize(denormalize(e)) == e;
+    {
+        MQ.Nth_root_lemma();
+    }
+}
+
