crypto_specs/pow2.s.dfy
@@ -1,8 +1,8 @@
-include "../../std_lib/src/NonlinearArithmetic/Power2.dfy"
-include "../../std_lib/src/NonlinearArithmetic/DivMod.dfy"
-include "../../std_lib/src/Collections/Sequences/Seq.dfy"
+include "../std_lib/src/NonlinearArithmetic/Power2.dfy"
+include "../std_lib/src/NonlinearArithmetic/DivMod.dfy"
+include "../std_lib/src/Collections/Sequences/Seq.dfy"
 
-module pows_of_2 {
+module pow2_s {
     import opened Power
     import opened Power2
     import opened DivMod
@@ -32,20 +32,6 @@ module pows_of_2 {
         reveal Pow2();
     }
 
-    function method pow2_half(n: pow2_t) : (n': pow2_t)
-        requires n.exp != 0 || n.full != 1;
-        ensures n'.exp == n.exp - 1;
-        ensures n'.full * 2 == n.full;
-        ensures n.full % 2 == 0;
-        ensures n'.full == n.full / 2;
-    {
-        pow2_basics(n);
-        assert n.exp - 1 >= 0;
-        var m := pow2_t_cons(n.full / 2, n.exp - 1);
-        pow2_half_value_lemma(n, m);
-        m
-    }
-
     lemma pow2_half_value_lemma(n: pow2_t, n': pow2_t_raw)
         requires n.exp != 0;
         requires n' == pow2_t_cons(n.full / 2, n.exp - 1);
@@ -68,6 +54,20 @@ module pows_of_2 {
         }
     }
 
+    function method pow2_half(n: pow2_t) : (n': pow2_t)
+        requires n.exp != 0 || n.full != 1;
+        ensures n'.exp == n.exp - 1;
+        ensures n'.full * 2 == n.full;
+        ensures n.full % 2 == 0;
+        ensures n'.full == n.full / 2;
+    {
+        pow2_basics(n);
+        assert n.exp - 1 >= 0;
+        var m := pow2_t_cons(n.full / 2, n.exp - 1);
+        pow2_half_value_lemma(n, m);
+        m
+    }
+
     function method pow2_double(n: pow2_t) : (n': pow2_t)
         ensures n'.exp == n.exp + 1;
         ensures n'.full == n.full * 2;
@@ -82,8 +82,6 @@ module pows_of_2 {
     function method pow2_mul(n: pow2_t, m: pow2_t) : (n': pow2_t)
     {
         LemmaPowAdds(2, n.exp, m.exp);
-        // LemmaPowAdds(2, m.exp, n.exp);
-        // LemmaMulIsCommutative(n.full, m.full);
         LemmaMulStrictlyPositiveAuto();
         reveal Pow2();
         var a := pow2_t_cons(n.full * m.full, n.exp + m.exp);
@@ -106,25 +104,4 @@ module pows_of_2 {
         LemmaFundamentalDivMod(n.full, m.full);
         a
     }
-
-    // lemma pow2_square(n: pow2_t) returns (n': pow2_t)
-    //     ensures n'.exp == 2 * n.exp 
-    //     ensures n'.full == n.full * n.full
-    // {
-    //     LemmaMulStrictlyPositiveAuto();
-    //     var m := pow2_t_cons(n.full * n.full, 2 * n.exp);
-
-    //     calc == {
-    //         m.full;
-    //         n.full * n.full;
-    //         Pow2(n.exp) * Pow2(n.exp);
-    //         {
-    //             LemmaPowAdds(2, n.exp, n.exp);
-    //         }
-    //         Pow2(n.exp + n.exp);
-    //         Pow2(m.exp);
-    //     }
-
-    //     n' := m;
-    // }
 }
